SL_Core_Soundness.v
@@ -1,0 +1,483 @@
+(***************************************************************************
+* Safety for Lambda Mu Mutilde (CBV) - Infrastructure                      *
+* Étienne Miquey, June 2015                                                *
+***************************************************************************)
+
+Set Implicit Arguments.
+Require Import LibLN 
+  L_Core_Definitions 
+  L_Core_Infrastructure
+  L_Core_Soundness.
+Require Import SL_Core_Definitions.
+
+
+(* ********************************************************************** *)
+(** * Proofs *)
+
+(** Typing is preserved by weakening. *)
+
+
+(*Scheme typing_prf_ind := Induction for typing_prf Sort Prop
+  with typing_cont_ind := Induction for typing_cont Sort Prop
+  with typing_clos_ind := Induction for typing_clos Sort Prop.
+
+Combined Scheme typing_mut_ind from typing_prf_ind,typing_cont_ind,typing_clos_ind.
+ *)
+
+Fixpoint typing_sprf_weaken A tau p T (H: typing_sprf A tau p T) {struct H}:
+  forall E F G, A=E&G -> ok (E & F & G) ->  typing_sprf  (E & F & G) tau p T
+with typing_scont_weaken A tau e T (H:typing_scont A tau e T) {struct H}:
+  forall E F G, A=E&G ->  ok (E & F & G) -> typing_scont (E & F & G) tau e T
+with typing_sclos_weaken A tau c  (H: typing_sclos A tau c) {struct H}:
+  forall E F G, A=E&G -> ok (E & F & G) -> typing_sclos (E & F & G) tau c .
+Proof.
+  induction H; intros.
+  + apply* typing_sprf_var.
+    apply* binds_weaken.
+    subst.
+    assumption.
+  + apply typing_store_var.
+    destruct H as (q,(l,(Hl,(Binds,HI)))).
+    exists q l;repeat split*.
+ +  apply_fresh typing_abs.
+    rewrite <- concat_assoc.
+    apply* H0.
+    symmetry.
+    subst.
+    apply concat_assoc.
+    rewrite concat_assoc.
+    apply* ok_push.
+ +  apply_fresh (@typing_mu). 
+    rewrite <- concat_assoc.
+    apply (typing_sclos_weaken (E0 & (G & y ~ neg T))).
+    rewrite  concat_assoc.
+    subst.
+    apply* H.
+    reflexivity.
+    rewrite concat_assoc.
+    apply* ok_push.
+ +
+    
+
+    
+    Guarded.
+Lemma typing_store_weaken :
+  (  forall A tau p T (H: typing_sprf A tau p T) E F G,
+       A=E&G -> 
+       ok (E & F & G) ->  typing_sprf  (E & F & G) tau p T)
+/\ (forall A tau e T (H:typing_scont A tau e T) E F G,
+A=E&G ->  ok (E & F & G) -> typing_scont (E & F & G) tau e T)
+/\ (forall A tau c  (H: typing_sclos A tau c) E F G,
+ A=E&G -> ok (E & F & G) -> typing_sclos (E & F & G) tau c) .
+Proof.
+  apply (typing_store_mut_ind).
+  + intros A tau a T OkA Binds E F G HA Ok.
+    apply* typing_sprf_var. apply* binds_weaken.
+    rewrite HA in Binds.
+    assumption.
+  + intros A tau a T (q,(l,(Hl,(Binds,Hq)))) E F G HE Ok.
+    apply* typing_store_var.
+    exists q l;repeat split*. 
+    apply* binds_weaken.
+    rewrite HA in Binds.
+    assumption.
+  + intros L A U T p Ha IH E F G HA Ok.
+    apply_fresh typing_abs.
+    rewrite <- concat_assoc.
+    apply* IH.
+    rewrite HA.
+    rewrite <-concat_assoc.
+    reflexivity.
+    rewrite concat_assoc.
+    apply* ok_push.
+  + intros L A T c Ha IH E F G HA Ok.
+    apply_fresh (@typing_mu). 
+    rewrite <- concat_assoc.
+    apply* (IH y) .
+    rewrite HA.
+    rewrite <- concat_assoc.
+    reflexivity.
+    rewrite concat_assoc.
+    apply* ok_push.
+  + intros A a T OkA Binds E F G HA Ok.     
+    apply* typing_cont_var.
+    rewrite HA in Binds.
+    apply* binds_weaken.
+  + intros L A T c Ha IH E F G HA Ok.
+    apply_fresh typing_mut.
+    rewrite <- concat_assoc.
+    apply* (IH y).
+    rewrite concat_assoc.
+    rewrite* HA.
+    rewrite concat_assoc.
+    apply* ok_push. 
+  + intros A U T q e Hq IHq He IHe E F G HA Ok.
+    apply* typing_stack.
+  + intros A T p e Hp IHp He IHe E F G HA Ok.
+    rewrite HA in *.
+    apply (@typing_closure (E&F&G) T); [apply* IHp|apply* IHe].
+Qed.    
+
+
+Lemma typing_prf_weaken: forall G E F p T,
+ (E & G) |= p :+ T -> ok (E & F & G) ->  (E & F & G) |= p :+ T.
+Proof.
+  destruct typing_weaken as [Hp _ ].
+  intros;apply* Hp.
+Qed.
+
+Lemma typing_cont_weaken: forall  G E F e T,
+ (E & G) |= e :- T -> ok (E & F & G) ->   (E & F & G) |= e :- T.
+Proof.
+  destruct typing_weaken as [_ (He,_ )].
+  intros;apply* He.
+Qed.
+
+Lemma typing_clos_weaken: forall G E F c,
+c:*(E & G) ->  ok (E & F & G) ->   c:* (E & F & G) .
+Proof.
+  destruct typing_weaken as [_ (_,Hc)].
+  intros;apply* Hc.
+Qed.
+
+(** Typing is preserved by substitution. *)
+
+Lemma typing_subst_prf:
+  (forall  A  p T (H: A |= p:+ T) F U E z q,
+     A=(E & z ~ pos U & F) -> E |= q :+ U -> (E & F) |= [z ~+> q]+ p :+ T)
+  /\(forall A e T (H: A |= e:- T ) F U E z q,
+   A=(E & z ~ pos U & F)   ->   E |= q :+ U -> (E & F) |= [z ~+> q]- e :- T)
+/\(forall A c (H: c:* A) F U E  z q, 
+ A=(E & z ~ pos U & F) ->  E |= q :+ U -> [z ~+> q]* c :* (E&F)).
+Proof.
+  apply typing_mut_ind.
+  - intros A a T Ok Binds F U E z q HA Typq.
+    rewrite HA in *;simpl.
+    + case_var.
+      * apply binds_middle_eq_inv in Binds.
+        inversion Binds.
+        apply_empty* typing_prf_weaken.
+        assumption.
+      * apply* typing_prf_var.
+        apply* binds_subst.
+  - intros L A U T p Hp IH F T' E z q HA Typq.
+    rewrite HA in *;simpl.
+    apply_fresh typing_abs.
+    rewrite* subst_open_prf_prf_var.
+    rewrite <- concat_assoc.
+    apply* IH.
+    rewrite* <- concat_assoc.
+  - intros L A T c Hc IH F U E z q HA Typq.
+    rewrite HA in *;simpl.
+    apply_fresh typing_mu.
+    rewrite <- concat_assoc.
+    assert (y \notin L) by intuition.
+    rewrite subst_open_clos_prf_var1.
+    + apply (IH y H _ U).
+      * rewrite* concat_assoc.
+      * assumption.
+    + apply* notin_singleton.
+    + destruct* (typing_regular_prf Typq).
+   - intros A a T Ok Binds F U E z q HA Typq.
+    rewrite HA in *;simpl.
+    apply* typing_cont_var.
+    destruct*  (binds_middle_inv Binds).
+    destruct* H.
+    intuition.
+    inversion H2.
+  - intros L A T c Hc IH F T' E z q HA Typq.
+    rewrite HA in *;simpl.
+    apply_fresh typing_mut.
+    rewrite <- concat_assoc.
+    assert (y \notin L) by intuition.
+    rewrite subst_open_clos_prf_var.
+    + apply* IH.
+      rewrite* concat_assoc.
+    + apply* notin_singleton.
+    + destruct* (typing_regular_prf Typq).
+  - intros A U T p e Hp IHp He IHe F T' E z q HA Typq.
+    rewrite HA in *;simpl.
+    apply typing_stack.
+    + apply* IHp.
+    + apply* IHe.
+  - intros A T p e Hp IHp He IHe F U E z q HA Typq.
+    rewrite HA in *;simpl.
+    apply (@typing_closure (E&F) T).    
+    * apply* IHp.
+    * apply* IHe.
+Qed.
+
+(* Splitting this in three pieces *)
+
+Lemma typing_prf_subst_prf:
+  forall F U E p T z q,((E & z ~ pos U & F) |= p:+ T) ->
+  E |= q :+ U -> (E & F) |= [z ~+> q]+ p :+ T.
+Proof.
+destruct typing_subst_prf as [Hp _ ].
+intros;apply* Hp.
+Qed.
+
+Lemma typing_cont_subst_prf:
+  forall F U E e T z q, (E & z ~ pos U & F) |= e:- T ->
+  E |= q :+ U -> (E & F) |= [z ~+> q]- e :- T.
+Proof.
+  destruct typing_subst_prf as [_ (He,_)].
+  intros;apply* He.
+Qed.
+  
+Lemma typing_clos_subst_prf:
+  forall F U E c z q, (c:* (E & z ~ pos U & F))->
+   E |= q :+ U -> [z ~+> q]* c :* (E&F).
+Proof.
+  destruct typing_subst_prf as [_ (_,Hc) ].
+  intros;apply* Hc.
+Qed.
+(* negative version *)
+
+Lemma typing_subst_cont:
+  (forall  A  p T (H: A |= p:+ T) F U E z f,
+     A=(E & z ~ (neg U) & F) -> E |= f :- U -> (E & F) |= [z ~-> f]+ p :+ T)
+  /\(forall A e T (H: A |= e:- T ) F U E z f,
+   A=(E & z ~ (neg U) & F)   ->   E |= f :- U -> (E & F) |= [z ~-> f]- e :- T)
+/\(forall A c (H: c:* A) F U E  z f, 
+ A=(E & z ~ (neg U) & F) ->  E |= f :- U -> [z ~-> f]* c :* (E&F)).
+Proof.
+  apply typing_mut_ind.
+  - intros A a T Ok Binds F U E z q HA Typq.
+    rewrite HA in *;simpl.
+    + apply* typing_prf_var.
+      destruct* (binds_middle_inv Binds).
+      destruct* H.
+      destruct H as [_ (_,H)].
+      inversion H.
+  - intros L A U T p Hp IH F T' E z q HA Typq.
+    rewrite HA in *;simpl.
+    apply_fresh typing_abs.
+    rewrite* subst_open_prf_cont_var1.
+    rewrite <- concat_assoc.
+    apply* IH.
+    rewrite* <- concat_assoc.
+  - intros L A T c Hc IH F U E z q HA Typq.
+    rewrite HA in *;simpl.
+    apply_fresh typing_mu.
+    rewrite <- concat_assoc.
+    assert (y \notin L) by intuition.
+    rewrite subst_open_clos_cont_var.
+    + apply (IH y H _ U).
+      * rewrite* concat_assoc.
+      * assumption.
+    + apply* notin_singleton.
+    + destruct* (typing_regular_cont Typq).
+   - intros A a T Ok Binds F U E z q HA Typq.
+    rewrite HA in *;simpl.
+    case_var.
+     * apply binds_middle_eq_inv in Binds.
+       inversion Binds.
+       apply_empty* typing_cont_weaken.
+       assumption.
+     * apply* typing_cont_var.
+       apply* binds_subst.
+  - intros L A T c Hc IH F T' E z q HA Typq.
+    rewrite HA in *;simpl.
+    apply_fresh typing_mut.
+    rewrite <- concat_assoc.
+    assert (y \notin L) by intuition.
+    rewrite subst_open_clos_cont_var1.
+    + apply* IH.
+      rewrite* concat_assoc.
+    + apply* notin_singleton.
+    + destruct* (typing_regular_cont Typq).
+  - intros A U T p e Hp IHp He IHe F T' E z q HA Typq.
+    rewrite HA in *;simpl.
+    apply typing_stack.
+    + apply* IHp.
+    + apply* IHe.
+  - intros A T p e Hp IHp He IHe F U E z q HA Typq.
+    rewrite HA in *;simpl.
+    apply (@typing_closure (E&F) T).    
+    * apply* IHp.
+    * apply* IHe.
+Qed.
+
+
+
+(* Splitting this in three pieces *)
+
+Lemma typing_prf_subst_cont:
+  forall F U E p T z f,((E & z ~ (neg U) & F) |= p:+ T) ->
+  E |= f :-  U -> (E & F) |= [z ~-> f]+ p :+ T.
+Proof.
+destruct typing_subst_cont as [Hp _ ].
+intros;apply* Hp.
+Qed.
+
+Lemma typing_cont_subst_cont:
+  forall F U E e T z f, (E & z ~  (neg U) & F) |= e:- T ->
+  E |= f :-  U -> (E & F) |= [z ~-> f]- e :- T.
+Proof.
+  destruct typing_subst_cont as [_ (He,_)].
+  intros;apply* He.
+Qed.
+  
+Lemma typing_clos_subst_cont:
+  forall F U E c z f, (c:* (E & z ~  (neg U) & F))->
+   E |= f :-  U -> [z ~-> f]* c :* (E&F).
+Proof.
+  destruct typing_subst_cont as [_ (_,Hc) ].
+  intros;apply* Hc.
+Qed.
+
+
+
+
+(** Preservation (typing is preserved by reduction). *)
+
+Lemma open_clos_comm: forall p e y,  cl p e *^+ y = cl (p+^+y) (e-^+y).
+Proof.
+  intros.
+  reflexivity.
+Qed.
+
+Lemma open_cont_proof_def : forall e y, e-^+y = {0 ~+> (prf_fvar y)}-e.  
+Proof.
+  intros;reflexivity.
+Qed.
+
+Lemma subject_reduction : preservation.
+Proof.
+  introv Typ. gen c'.
+  inductions Typ;intros c Red;inversions Red.
+  - inversions H0.
+    inversion H3.
+    pick_fresh x.
+    rewrite* (@subst_intro_clos_prf x).
+    apply_empty* typing_clos_subst_prf.
+  - inversion H0.
+    apply* (@typing_closure E T0).
+    rewrite <-  H8 in *.
+    inversion H.
+    apply_fresh typing_mut.
+    simpl.
+    assert (y\notin L) by intuition.
+    rewrite open_clos_comm.
+    apply (@typing_closure (E&y~pos T0) U).
+    + apply* H13.
+    + destruct (typing_regular_cont H9).
+      rewrite open_cont_proof_def.
+      rewrite* <-(open_rec_cont_prf_id).
+      apply_empty* typing_cont_weaken.
+  - inversion H.
+    pick_fresh x.
+    rewrite* (@subst_intro_clos_cont x).
+    apply_empty* typing_clos_subst_cont.  
+Qed.
+
+(** Progress (a well-typed term is either a value or it can 
+  take a step of reduction). *)
+
+
+Lemma progress_one_step :
+  (forall E (p : prf) (T : typ),
+     E |= p :+ T -> E=empty ->
+     value p \/(exists L,forall a, a\notin L -> exists c, red (cl p (co_fvar a)) (c)))
+(*/\ (forall E (e:cont) (T : typ),
+      E |= e :- T -> E=empty -> True)
+/\ (forall E (c : clos) ,c :* E ->
+   (E=empty -> True))*)
+.
+Proof.
+  intros E p T Hp.
+  induction Hp.
+  -intros HE.
+   rewrite HE in *.
+   false* binds_empty_inv.
+  - intros HE.
+  left*.
+  apply value_abs.
+  apply (@proof_abs L).
+  intros.
+  specialize (H a H1).
+  destruct* (typing_regular_prf H).
+- intros HE.
+  right.
+  exists L.
+  intros a Ha.
+  exists (c*^-a).
+  apply* red_mu.
+  apply_fresh proof_mu.
+  assert (y\notin L) as Hy by intuition.
+  specialize (H y Hy).
+  apply (typing_regular_clos) in H.
+  destruct* H.
+Qed.
+
+
+
+
+
+
+
+(*  
+Lemma progress_result :
+  (forall E (p : prf) (T : typ),
+     E |= p :+ T -> E=empty ->
+     value p \/(exists L,forall a, a\notin L -> exists p' n, redn n (cl p (co_fvar a)) (cl p' (co_fvar a))))
+/\ (forall E (e:cont) (T : typ),
+      E |= e :- T -> E=empty -> True)
+/\ (forall E (c : clos) ,c :* E ->
+  forall a T, E=a~neg T ->exists p' n,  (redn n c (cl p' (co_fvar a))\/ c = cl p' (co_fvar a)) /\ E |= p' :+ T)
+.
+Proof.
+  apply typing_mut_ind.
+- intros E p T Ok Binds HE.
+  rewrite HE in *.
+  false* binds_empty_inv.
+- intros L E U T p Hp IH  HE.
+  rewrite HE in *.
+  left*.
+  apply value_abs.
+  apply (@proof_abs L).
+  intros.
+  specialize (Hp a H).
+  destruct* (typing_regular_prf Hp).
+- intros L E T c Hc IH HE.
+  rewrite HE in *.
+  right.
+  exists L.
+  intros a Ha.
+  destruct* (IH a Ha a T (concat_empty_l (a~neg T))) as (p',(n,([Red|Eq],Typ))).
+  + exists p' (n+1).
+    apply redS.
+    exists (c *^-a).
+    split.
+    * apply* red_mu.
+      apply_fresh proof_mu.
+      assert (y\notin L) as Hy by intuition.
+      specialize (Hc y Hy).
+      apply (typing_regular_clos) in Hc.
+      destruct* Hc as (_,Ok).
+    * assumption.
+  + exists p' 1.
+    apply red1.        
+    rewrite <- Eq.
+    apply* red_mu.
+    apply_fresh proof_mu.
+    assert (y\notin L) as Hy by intuition.
+    specialize (Hc y Hy).
+    apply (typing_regular_clos) in Hc.
+    destruct* Hc as (_,Ok).
+- tauto.
+- tauto.
+- tauto.
+- intros E T p e Hp IHp He _ a U HE.
+  rewrite HE in *.
+  inversion He.
+  + apply binds_single_inv in H0.
+    destruct H0.
+    inversion H4.
+    subst.
+    exists p 0.
+    split~.
+    + admit.
+  + subst.
+*)
